added improved version

CRDT/ORSet2.thy
@@ -15,138 +15,79 @@ imports
   Network
 begin
 
-datatype ('id, 'a, 'b) operation = Add "'id" "'a" | Rem "'id set" "'a" "'b set" | Append "'a" "'b" |
-	Store "'a" "'b" "'b"
+datatype ('id, 'a) operation = Add "'id" "'a" | Rem "'id set" "'a" | Store "'a" "'id" "'id"
 
-type_synonym ('id, 'a, 'b) state = "('a \<Rightarrow> 'id set) \<times> ('a \<rightharpoonup> 'b set)"
+type_synonym ('id, 'a) state = "'a \<rightharpoonup> 'id set"
 
-definition op_elem :: "('id, 'a, 'b) operation \<Rightarrow> 'a" where
-  "op_elem oper \<equiv> case oper of Add i e \<Rightarrow> e | Rem is e m \<Rightarrow> e | Append e m \<Rightarrow> e | Store e mo mn \<Rightarrow> e"
-		
-definition interpret_op :: "('id, 'a, 'b) operation \<Rightarrow> ('id, 'a, 'b) state \<rightharpoonup> ('id, 'a, 'b) state" ("\<langle>_\<rangle>" [0] 1000) where
+definition op_elem :: "('id, 'a) operation \<Rightarrow> 'a" where
+  "op_elem oper \<equiv> case oper of Add i e \<Rightarrow> e | Rem is e \<Rightarrow> e | Store e mo mn \<Rightarrow> e"
+
+definition interpret_op :: "('id, 'a) operation \<Rightarrow> ('id, 'a) state \<rightharpoonup> ('id, 'a) state" ("\<langle>_\<rangle>" [0] 1000) where
   "interpret_op oper state \<equiv>
-     let before = ((fst state) (op_elem oper));
-         after  = case oper of Add i e \<Rightarrow> before \<union> {i} | Rem is e m \<Rightarrow> before - is | Append e m \<Rightarrow> before | Store e mo mn \<Rightarrow> before;
-         filesystem = case oper of 
-           Add i e \<Rightarrow> (case snd state e of None \<Rightarrow> Some {} | Some f \<Rightarrow> Some f) | 
-           Rem is e m \<Rightarrow> (case snd state e of None \<Rightarrow> None | Some f \<Rightarrow> Some (f - m)) |
-					 Append e m \<Rightarrow> (case snd state e of None \<Rightarrow> None | Some f \<Rightarrow> Some (insert m f)) |
-					 Store e mo mn \<Rightarrow> (case snd state e of None \<Rightarrow> None | Some f \<Rightarrow> Some (insert mn (f - {mo})))
-     in  Some ((fst state) ((op_elem oper) := after), (snd state) ((op_elem oper) := filesystem))"
+     let mailbox  = case oper of 
+		   Add i e \<Rightarrow> (case state e of None \<Rightarrow> Some {i} | Some f \<Rightarrow> Some (insert i f)) | 
+       Rem is e \<Rightarrow> (case state e of None \<Rightarrow> None | Some f \<Rightarrow> (case f - is = {} of True \<Rightarrow> None | False \<Rightarrow> Some (f - is))) |
+       Store e mo mn \<Rightarrow> (case state e of None \<Rightarrow> Some {mn} | Some f \<Rightarrow> Some (insert mn (f - {mo})))
+     in  Some (state ((op_elem oper) := mailbox))"
   
-definition valid_behaviours :: "('id, 'a, 'b) state \<Rightarrow> 'id \<times> ('id, 'a, 'b) operation \<Rightarrow> bool" where
+definition valid_behaviours :: "('id, 'a) state \<Rightarrow> 'id \<times> ('id, 'a) operation \<Rightarrow> bool" where
   "valid_behaviours state msg \<equiv>
      case msg of
-       (i, Add j e) \<Rightarrow> i = j|
-       (i, Rem is e m) \<Rightarrow> is = fst state e"
+       (i, Add j e) \<Rightarrow> i = j |
+       (i, Rem is e) \<Rightarrow> (case state e of None \<Rightarrow> False | Some f \<Rightarrow> is = f) |
+       (i, Store e mo mn) \<Rightarrow> i = mn"
 
-locale orset = network_with_constrained_ops _ interpret_op "(\<lambda>x. {}, \<lambda>y. None)" valid_behaviours
+locale orset = network_with_constrained_ops _ interpret_op "\<lambda>x. None" valid_behaviours
 
-lemma (in orset) add_add_commute:
-  shows "\<langle>Add i1 e1\<rangle> \<rhd> \<langle>Add i2 e2\<rangle> = \<langle>Add i2 e2\<rangle> \<rhd> \<langle>Add i1 e1\<rangle>"
-  by(auto simp add: interpret_op_def op_elem_def kleisli_def, fastforce)
+lemma add_add_commute:
+  shows "(\<langle>Add i1 e1\<rangle> \<rhd> \<langle>Add i2 e2\<rangle>) s = (\<langle>Add i2 e2\<rangle> \<rhd> \<langle>Add i1 e1\<rangle>) s"
+  	unfolding interpret_op_def op_elem_def kleisli_def  apply (case_tac "e1=e2") apply simp apply auto
+  	by (simp add: insert_commute option.case_eq_if)
 
-lemma (in orset) add_rem_commute2:
-  fixes s
-  assumes "i \<notin> is"  and "e1 \<noteq> e2"
-  shows " (\<langle>Add i e1\<rangle> \<rhd> \<langle>Rem is e2 m\<rangle>) s = (\<langle>Rem is e2 m\<rangle> \<rhd> \<langle>Add i e1\<rangle>) s"
-  	unfolding interpret_op_def op_elem_def kleisli_def using assms apply simp
-  	by (smt fun_upd_other fun_upd_twist snd_conv)
- 
-lemma (in orset) add_rem_commute3:
-  fixes s
+lemma add_rem_commute:
   assumes "i \<notin> is"
-  shows " (\<langle>Add i e\<rangle> \<rhd> \<langle>Rem is e m\<rangle>) s = (\<langle>Rem is e m\<rangle> \<rhd> \<langle>Add i e\<rangle>) s"
-  	unfolding interpret_op_def op_elem_def kleisli_def using assms apply simp
-  	by (simp add: insert_Diff_if option.case_eq_if)
-  	
-lemma (in orset) add_rem_commute:
-  assumes "i \<notin> is" 
-  shows "\<langle>Add i e1\<rangle> \<rhd> \<langle>Rem is e2 m\<rangle> = \<langle>Rem is e2 m\<rangle> \<rhd> \<langle>Add i e1\<rangle>"
-proof 
-	fix x
-	show "(\<langle>Add i e1\<rangle> \<rhd> \<langle>Rem is e2 m\<rangle>) x = (\<langle>Rem is e2 m\<rangle> \<rhd> \<langle>Add i e1\<rangle>) x "
-		using assms add_rem_commute3[of "i" "is" "e1" "m" x] add_rem_commute2 [of "i" "is" "e1" "e2" "m" "x"]
-		by auto
-qed
-  	
-lemma rem_rem_commute1:
-assumes "e1 \<noteq> e2"
-shows " (\<langle>Rem i1 e1 m1\<rangle> \<rhd> \<langle>Rem i2 e2 m2\<rangle>) s = (\<langle>Rem i2 e2 m2\<rangle> \<rhd> \<langle>Rem i1 e1 m1\<rangle>) s"
-unfolding interpret_op_def kleisli_def op_elem_def using assms by (simp add: fun_upd_twist)
-  	
-lemma rem_rem_commute2:
-assumes "(snd s) e1 = None"
-shows " (\<langle>Rem i1 e1 m1\<rangle> \<rhd> \<langle>Rem i2 e1 m2\<rangle>) s = (\<langle>Rem i2 e1 m2\<rangle> \<rhd> \<langle>Rem i1 e1 m1\<rangle>) s"
-unfolding interpret_op_def kleisli_def op_elem_def using assms apply simp by fastforce
-    	
-lemma rem_rem_commute3:
-assumes "(snd s) e1 \<noteq> None"
-shows " (\<langle>Rem i1 e1 m1\<rangle> \<rhd> \<langle>Rem i2 e1 m2\<rangle>) s = (\<langle>Rem i2 e1 m2\<rangle> \<rhd> \<langle>Rem i1 e1 m1\<rangle>) s"
-unfolding interpret_op_def kleisli_def op_elem_def apply simp 
-proof
-	show "(fst s)(e1 := fst s e1 - i1 - i2) = (fst s)(e1 := fst s e1 - i2 - i1)" by fastforce
-	show "(snd s)(e1 := case case snd s e1 of None \<Rightarrow> None | Some f \<Rightarrow> Some (f - m1) of None \<Rightarrow> None | Some f \<Rightarrow> Some (f - m2)) = (snd s)
-		(e1 := case case snd s e1 of None \<Rightarrow> None | Some f \<Rightarrow> Some (f - m2) of None \<Rightarrow> None | Some f \<Rightarrow> Some (f - m1))" 
-		using assms apply simp by auto 
-qed
-	
+  shows "(\<langle>Add i e1\<rangle> \<rhd> \<langle>Rem is e2\<rangle>) s = (\<langle>Rem is e2\<rangle> \<rhd> \<langle>Add i e1\<rangle>) s"
+  using assms unfolding interpret_op_def kleisli_def op_elem_def apply (case_tac "e1=e2") apply simp apply auto
+  	apply (simp add:  insert_Diff_if option.case_eq_if option.discI )
+  by (smt option.discI Diff_eq_empty_iff option.sel)
+ 
 lemma rem_rem_commute:
-shows " \<langle>Rem i1 e1 m1\<rangle> \<rhd> \<langle>Rem i2 e2 m2\<rangle> = \<langle>Rem i2 e2 m2\<rangle> \<rhd> \<langle>Rem i1 e1 m1\<rangle>"
-proof
-	fix x
-	show "(\<langle>Rem i1 e1 m1\<rangle> \<rhd> \<langle>Rem i2 e2 m2\<rangle>) x = (\<langle>Rem i2 e2 m2\<rangle> \<rhd> \<langle>Rem i1 e1 m1\<rangle>) x"
-		using rem_rem_commute1[of e1 e2 i1 m1 i2 m2 x] 
-				  rem_rem_commute2[of x e1 i1 m1 i2 m2] 
-          rem_rem_commute3[of x e1 i1 m1 i2 m2]
-    by auto
-qed 
+  shows "(\<langle>Rem i1 e1\<rangle> \<rhd> \<langle>Rem i2 e2\<rangle>) s = (\<langle>Rem i2 e2\<rangle> \<rhd> \<langle>Rem i1 e1\<rangle>) s"
+  unfolding interpret_op_def op_elem_def kleisli_def apply (case_tac "e1=e2") apply simp apply auto
+  apply	(case_tac "s e2 = None") proof(auto)
+  fix y
+  show "e1 = e2 \<Longrightarrow>
+         s e2 = Some y \<Longrightarrow>
+         s(e2 := case case y \<subseteq> i1 of True \<Rightarrow> None | False \<Rightarrow> Some (y - i1) of None \<Rightarrow> None
+                 | Some f \<Rightarrow> case f - i2 = {} of True \<Rightarrow> None | False \<Rightarrow> Some (f - i2)) =
+         s(e2 := case case y \<subseteq> i2 of True \<Rightarrow> None | False \<Rightarrow> Some (y - i2) of None \<Rightarrow> None
+                 | Some f \<Rightarrow> case f - i1 = {} of True \<Rightarrow> None | False \<Rightarrow> Some (f - i1))"	
+    apply (case_tac "y \<subseteq> i1") apply auto 
+     apply (smt Diff_eq_empty_iff Diff_subset option.case_eq_if option.sel subset_trans) sorry
+      qed
+      (*by (smt Diff_Int2 Diff_Int_distrib2 Diff_eq Diff_eq_empty_iff Diff_subset option.simps(4) option.simps(5)) *)
+  	
 
-lemma append_append_commute:
-shows " \<langle>Append e1 m1\<rangle> \<rhd> \<langle>Append e2 m2\<rangle> = \<langle>Append e2 m2\<rangle> \<rhd> \<langle>Append e1 m1\<rangle>"
-proof
-	fix x
-	show "(\<langle>Append e1 m1\<rangle> \<rhd> \<langle>Append e2 m2\<rangle>) x = (\<langle>Append e2 m2\<rangle> \<rhd> \<langle>Append e1 m1\<rangle>) x"
-		unfolding interpret_op_def kleisli_def op_elem_def apply simp
-		by (simp add: fun_upd_twist insert_commute option.case_eq_if)
-qed  
-
-lemma add_append_commute:
-	assumes "(snd x) e2 \<noteq> None"
-	shows " (\<langle>Add i e1\<rangle> \<rhd> \<langle>Append e2 m2\<rangle>) x = (\<langle>Append e2 m2\<rangle> \<rhd> \<langle>Add i e1\<rangle>) x"
-		unfolding interpret_op_def kleisli_def op_elem_def apply simp
-		by (simp add: assms fun_upd_twist option.case_eq_if)
-			
-lemma rem_append_commute:
-	assumes  "m2 \<notin> m1"
-	shows " (\<langle>Rem is e1 m1\<rangle> \<rhd> \<langle>Append e2 m2\<rangle>) x = (\<langle>Append e2 m2\<rangle> \<rhd> \<langle>Rem is e1 m1\<rangle>) x"
-		unfolding interpret_op_def kleisli_def op_elem_def apply simp using assms
-		by (simp add: assms(1) fun_upd_twist insert_Diff_if option.case_eq_if)
-			
+lemma rem_store_commute:
+	assumes "mn \<notin> is"
+  shows "(\<langle>Store e1 mo mn\<rangle> \<rhd> \<langle>Rem is e2\<rangle>) s = (\<langle>Rem is e2\<rangle> \<rhd> \<langle>Store e1 mo mn\<rangle>) s"
+  unfolding interpret_op_def kleisli_def op_elem_def apply (case_tac "e1=e2") apply simp apply auto
+  apply	(case_tac "s e2 = None") apply auto apply (simp add: Diff_triv assms)
+  using assms 
+  by (smt Diff_eq_empty_iff Diff_insert Diff_insert0 Diff_insert2 insert_Diff insert_Diff_if option.case_eq_if option.discI option.sel)
+  	
+lemma add_store_commute:
+	assumes "mo \<noteq> i"
+  shows "(\<langle>Store e1 mo mn\<rangle> \<rhd> \<langle>Add i e2\<rangle>) s = (\<langle>Add i e2\<rangle> \<rhd> \<langle>Store e1 mo mn\<rangle>) s"
+  unfolding interpret_op_def kleisli_def op_elem_def apply (case_tac "e1=e2") apply simp apply auto	using assms
+  apply	(case_tac "s e2 = None") by auto
+  	
 lemma store_store_commute:
-	assumes "mn1 \<noteq> mo1" and "mn1 \<noteq> mo2" and "mn2 \<noteq> mo1" and "mn2 \<noteq> mo2"
-shows " (\<langle>Store e1 mo1 mn1\<rangle> \<rhd> \<langle>Store e2 mo2 mn2\<rangle>) x = (\<langle>Store e2 mo2 mn2\<rangle> \<rhd> \<langle>Store e1 mo1 mn1\<rangle>) x"
-	unfolding interpret_op_def kleisli_def op_elem_def apply (case_tac "e1=e2") apply simp apply auto using assms
-	by (smt Diff_insert insert_Diff_if insert_commute option.case_eq_if option.discI option.sel singletonD)
-		
-lemma store_add_commute:
-	assumes  "(snd x) e2 \<noteq> None"
-shows " (\<langle>Add i e1\<rangle> \<rhd> \<langle>Store e2 mo2 mn2\<rangle>) x = (\<langle>Store e2 mo2 mn2\<rangle> \<rhd> \<langle>Add i e1\<rangle>) x"
-	unfolding interpret_op_def kleisli_def op_elem_def apply (case_tac "e1=e2") apply simp apply auto
-	by (simp add: assms option.case_eq_if)
-
-lemma store_rem_commute:
-	assumes "mn2 \<notin> m"
-shows " (\<langle>Rem is e1 m\<rangle> \<rhd> \<langle>Store e2 mo2 mn2\<rangle>) x = (\<langle>Store e2 mo2 mn2\<rangle> \<rhd> \<langle>Rem is e1 m\<rangle>) x"
-	unfolding interpret_op_def kleisli_def op_elem_def apply (case_tac "e1=e2") apply simp apply auto
-	using assms by (smt Diff_insert Diff_insert2 insert_Diff_if option.case_eq_if option.simps(5))
-		
-lemma store_append_commute:
-	assumes "m \<noteq> mo2"
-shows " (\<langle>Append e1 m\<rangle> \<rhd> \<langle>Store e2 mo2 mn2\<rangle>) x = (\<langle>Store e2 mo2 mn2\<rangle> \<rhd> \<langle>Append e1 m\<rangle>) x"
-	unfolding interpret_op_def kleisli_def op_elem_def apply (case_tac "e1=e2") apply simp apply auto
-	by (simp add: assms insert_Diff_if insert_commute option.case_eq_if)
-		
+	assumes "mn1 \<noteq> mo2" and "mn2 \<noteq> mo1"
+  shows "(\<langle>Store e1 mo1 mn1\<rangle> \<rhd> \<langle>Store e2 mo2 mn2\<rangle>) s = (\<langle>Store e2 mo2 mn2\<rangle> \<rhd> \<langle>Store e1 mo1 mn1\<rangle>) s"
+  unfolding interpret_op_def kleisli_def op_elem_def apply (case_tac "e1=e2") apply simp apply auto	apply (case_tac "s e2 = None") apply auto 
+  using assms(1) assms(2) apply fastforce
+  using assms(1) assms(2) by fastforce
 
 lemma (in orset) apply_operations_never_fails:
   assumes "xs prefix of i"
@@ -158,7 +99,7 @@ using assms proof(induction xs rule: rev_induct, clarsimp)
       using snoc by force
   next
     case (Deliver e) thus ?thesis
-      using snoc by (simp, metis (no_types, lifting) bind.simps(2) interp_msg_def interpret_op_def prefix_of_appendD)
+      using snoc by (clarsimp, metis interpret_op_def interp_msg_def bind.bind_lunit prefix_of_appendD)
   qed
 qed
 
@@ -168,12 +109,12 @@ lemma (in orset) add_id_valid:
   shows "i1 = i2"
 proof -
   have "\<exists>s. valid_behaviours s (i1, Add i2 e)"
-    using assms deliver_in_prefix_is_valid unfolding valid_behaviours_def by fastforce
+    using assms deliver_in_prefix_is_valid by blast
   thus ?thesis
     by(simp add: valid_behaviours_def)
 qed
 
-definition (in orset) added_ids :: "('id \<times> ('id, 'b, 'c) operation) event list \<Rightarrow> 'b \<Rightarrow> 'id list" where
+definition (in orset) added_ids :: "('id \<times> ('id, 'b) operation) event list \<Rightarrow> 'b \<Rightarrow> 'id list" where
   "added_ids es p \<equiv> List.map_filter (\<lambda>x. case x of Deliver (i, Add j e) \<Rightarrow> if e = p then Some j else None | _ \<Rightarrow> None) es"
 
 lemma (in orset) [simp]:
@@ -189,7 +130,7 @@ lemma (in orset) added_ids_Broadcast_collapse [simp]:
   by (auto simp: added_ids_def map_filter_append map_filter_def)
     
 lemma (in orset) added_ids_Deliver_Rem_collapse [simp]:
-  shows "added_ids ([Deliver (i, Rem is e m)]) e' = []"
+  shows "added_ids ([Deliver (i, Rem is e)]) e' = []"
   by (auto simp: added_ids_def map_filter_append map_filter_def)
     
 lemma (in orset) added_ids_Deliver_Add_diff_collapse [simp]:
@@ -208,14 +149,10 @@ lemma (in orset) added_id_not_in_set:
 lemma (in orset) apply_operations_added_ids:
   assumes "es prefix of j"
     and "apply_operations es = Some f"
-  shows "fst f x \<subseteq> set (added_ids es x)"
+  shows "f x \<subseteq> set (added_ids es x)"
 using assms proof (induct es arbitrary: f rule: rev_induct, force)
   case (snoc x xs) thus ?case
-  proof (cases x)
-    case (Broadcast e)
-    moreover obtain a b where "e = (a, b)" by force
-    ultimately show ?thesis using snoc by (simp, blast)
-  next
+  proof (cases x, force)
     case (Deliver e)
     moreover obtain a b where "e = (a, b)" by force
     ultimately show ?thesis
@@ -237,20 +174,19 @@ using assms proof (induct xs rule: rev_induct, clarsimp)
       using snoc apply (case_tac b; clarsimp)
        apply (metis added_ids_Deliver_Add_diff_collapse added_ids_Deliver_Add_same_collapse
               empty_iff list.set(1) set_ConsD add_id_valid in_set_conv_decomp prefix_of_appendD)
-       apply force
-        sorry
-       (*done *) 
+      apply force
+      done  
   qed
 qed
 
 lemma (in orset) Broadcast_Deliver_prefix_closed:
-  assumes "xs @ [Broadcast (r, Rem ix e m)] prefix of j"
+  assumes "xs @ [Broadcast (r, Rem ix e)] prefix of j"
     and "i \<in> ix"
   shows "Deliver (i, Add i e) \<in> set xs"
 proof -  
   obtain y where "apply_operations xs = Some y"
     using assms broadcast_only_valid_msgs by blast
-  moreover hence "ix = fst y e"
+  moreover hence "ix = y e"
     by (metis (mono_tags, lifting) assms(1) broadcast_only_valid_msgs operation.case(2) option.simps(1)
      valid_behaviours_def case_prodD)
   ultimately show ?thesis
@@ -259,7 +195,7 @@ qed
 
 lemma (in orset) Broadcast_Deliver_prefix_closed2:
   assumes "xs prefix of j"
-    and "Broadcast (r, Rem ix e m) \<in> set xs"
+    and "Broadcast (r, Rem ix e) \<in> set xs"
     and "i \<in> ix"
   shows "Deliver (i, Add i e) \<in> set xs"
 using assms Broadcast_Deliver_prefix_closed by (induction xs rule: rev_induct; force)
@@ -267,10 +203,10 @@ using assms Broadcast_Deliver_prefix_closed by (induction xs rule: rev_induct; f
 lemma (in orset) concurrent_add_remove_independent_technical:
   assumes "i \<in> is"
     and "xs prefix of j"
-    and "(i, Add i e) \<in> set (node_deliver_messages xs)" and "(ir, Rem is e m) \<in> set (node_deliver_messages xs)"
-  shows "hb (i, Add i e) (ir, Rem is e m)"
+    and "(i, Add i e) \<in> set (node_deliver_messages xs)" and "(ir, Rem is e) \<in> set (node_deliver_messages xs)"
+  shows "hb (i, Add i e) (ir, Rem is e)"
 proof -
-  obtain pre k where "pre@[Broadcast (ir, Rem is e m)] prefix of k"
+  obtain pre k where "pre@[Broadcast (ir, Rem is e)] prefix of k"
     using assms delivery_has_a_cause events_before_exist prefix_msg_in_history by blast
   moreover hence "Deliver (i, Add i e) \<in> set pre"
     using Broadcast_Deliver_prefix_closed assms(1) by auto
@@ -293,10 +229,10 @@ qed
 lemma (in orset) ids_imply_messages_same:
   assumes "i \<in> is"
     and "xs prefix of j"
-    and "(i, Add i e1) \<in> set (node_deliver_messages xs)" and "(ir, Rem is e2 m) \<in> set (node_deliver_messages xs)"
+    and "(i, Add i e1) \<in> set (node_deliver_messages xs)" and "(ir, Rem is e2) \<in> set (node_deliver_messages xs)"
   shows "e1 = e2"
 proof -
-  obtain pre k where "pre@[Broadcast (ir, Rem is e2 m)] prefix of k"
+  obtain pre k where "pre@[Broadcast (ir, Rem is e2)] prefix of k"
     using assms delivery_has_a_cause events_before_exist prefix_msg_in_history by blast
   moreover hence "Deliver (i, Add i e2) \<in> set pre"
     using Broadcast_Deliver_prefix_closed assms(1) by blast
@@ -308,12 +244,12 @@ proof -
 qed
 
 corollary (in orset) concurrent_add_remove_independent:
-  assumes "\<not> hb (i, Add i e1) (ir, Rem is e2 m)" and "\<not> hb (ir, Rem is e2 m) (i, Add i e1)"
+  assumes "\<not> hb (i, Add i e1) (ir, Rem is e2)" and "\<not> hb (ir, Rem is e2) (i, Add i e1)"
     and "xs prefix of j"
-    and "(i, Add i e1) \<in> set (node_deliver_messages xs)" and "(ir, Rem is e2 m) \<in> set (node_deliver_messages xs)"
+    and "(i, Add i e1) \<in> set (node_deliver_messages xs)" and "(ir, Rem is e2) \<in> set (node_deliver_messages xs)"
   shows "i \<notin> is"
-  using assms ids_imply_messages_same concurrent_add_remove_independent_technical by fastforce  
-  	
+  using assms ids_imply_messages_same concurrent_add_remove_independent_technical by fastforce
+
 lemma (in orset) concurrent_operations_commute:
   assumes "xs prefix of i"
   shows "hb.concurrent_ops_commute (node_deliver_messages xs)"                     
@@ -324,12 +260,11 @@ proof -
            "hb.concurrent (a, b) (x, y)"
     hence "interp_msg (a, b) \<rhd> interp_msg (x, y) = interp_msg (x, y) \<rhd> interp_msg (a, b)"
       apply(unfold interp_msg_def, case_tac "b"; case_tac "y"; simp add: add_add_commute rem_rem_commute hb.concurrent_def)
-       apply (metis add_id_valid add_rem_commute assms concurrent_add_remove_independent prefix_contains_msg)+
+       apply (metis add_id_valid add_rem_commute assms concurrent_add_remove_independent hb.concurrentD1 hb.concurrentD2 prefix_contains_msg)+
       done
   } thus ?thesis
     by(fastforce simp: hb.concurrent_ops_commute_def)
 qed
-  
 
 theorem (in orset) convergence:
   assumes "set (node_deliver_messages xs) = set (node_deliver_messages ys)"
@@ -341,12 +276,14 @@ using assms by(auto simp add: apply_operations_def intro: hb.convergence_ext con
 context orset begin
 
 sublocale sec: strong_eventual_consistency weak_hb hb interp_msg
-  "\<lambda>ops.\<exists>xs i. xs prefix of i \<and> node_deliver_messages xs = ops" "(\<lambda>x.{}, \<lambda> x. None)"
+  "\<lambda>ops.\<exists>xs i. xs prefix of i \<and> node_deliver_messages xs = ops" "\<lambda>x.{}"
   apply(standard; clarsimp simp add: hb_consistent_prefix node_deliver_messages_distinct
         concurrent_operations_commute)
-  unfolding hb.apply_operations_def node_deliver_messages_def interp_msg_def apply simp
-    apply (meson interpret_op_def)
-    by (metis drop_last_message trivial_network.node_deliver_messages_def)
+   apply(metis (no_types, lifting) apply_operations_def bind.bind_lunit not_None_eq
+     hb.apply_operations_Snoc kleisli_def apply_operations_never_fails interp_msg_def)
+  using drop_last_message apply blast
+done
+
 end
 end
 
