CRDT/OR2.thy
@@ -1,0 +1,549 @@
+(* before shit broke loose
+*)
+(* Victor B. F. Gomes, University of Cambridge
+   Martin Kleppmann, University of Cambridge
+   Dominic P. Mulligan, University of Cambridge
+   Alastair R. Beresford, University of Cambridge
+*)
+
+section\<open>Observed-Remove Set\<close>
+ 
+text\<open>The ORSet is a well-known CRDT for implementing replicated sets, supporting two operations:
+     the \emph{insertion} and \emph{deletion} of an arbitrary element in the shared set.\<close>
+
+theory
+  OR2
+imports
+  Network
+begin
+
+datatype ('id, 'a) operation = Add "'id" "'a" | Rem "'id set" "'a" | Append "'a" "'id" |
+	Store "'a" "'id" "'id"
+
+type_synonym ('id, 'a) state = "('a \<Rightarrow> 'id set) \<times> ('a \<rightharpoonup> 'id set)"
+
+definition op_elem :: "('id, 'a) operation \<Rightarrow> 'a" where
+  "op_elem oper \<equiv> case oper of Add i e \<Rightarrow> e | Rem is e \<Rightarrow> e | Append e m \<Rightarrow> e | Store e mo mn \<Rightarrow> e"
+
+definition interpret_op :: "('id, 'a) operation \<Rightarrow> ('id, 'a) state \<rightharpoonup> ('id, 'a) state" ("\<langle>_\<rangle>" [0] 1000) where
+  "interpret_op oper state \<equiv>
+     let before = ((fst state) (op_elem oper));
+         metadata  = case oper of 
+           Add i e \<Rightarrow> before \<union> {i} | 
+           Rem is e \<Rightarrow> before - is | 
+           Append e i \<Rightarrow> before \<union> {i} | 
+           Store e mo mn \<Rightarrow> insert mn (before - {mo});
+         filesystem = case oper of 
+           Add i e \<Rightarrow> (case snd state e of None \<Rightarrow> Some {} | Some f \<Rightarrow> Some f) | 
+           Rem is e \<Rightarrow> (case snd state e of None \<Rightarrow> None | Some f \<Rightarrow> (case before - is = {} of True \<Rightarrow> None | False \<Rightarrow> Some(f - is))) |
+					 Append e m \<Rightarrow> (case snd state e of None \<Rightarrow> Some {m} | Some f \<Rightarrow> Some (insert m f)) |
+					 Store e mo mn \<Rightarrow> (case snd state e of None \<Rightarrow> Some {mn} | Some f \<Rightarrow> Some (insert mn (f - {mo})))
+     in  Some ((fst state) ((op_elem oper) := metadata), (snd state) ((op_elem oper) := filesystem))"
+  
+definition valid_behaviours :: "('id, 'a) state \<Rightarrow> 'id \<times> ('id, 'a) operation \<Rightarrow> bool" where
+  "valid_behaviours state msg \<equiv>
+     case msg of
+       (i, Add j e) \<Rightarrow> i = j |
+       (i, Rem is e) \<Rightarrow> is = fst state e |
+			 (i, Append e m) \<Rightarrow> i = m |
+			 (i, Store e mo mn) \<Rightarrow> i = mn"
+
+locale orset = network_with_constrained_ops _ interpret_op "(\<lambda>x. {}, \<lambda>y. None)" valid_behaviours
+
+lemma (in orset) add_add_commute:
+  shows "\<langle>Add i1 e1\<rangle> \<rhd> \<langle>Add i2 e2\<rangle> = \<langle>Add i2 e2\<rangle> \<rhd> \<langle>Add i1 e1\<rangle>"
+  by(auto simp add: interpret_op_def op_elem_def kleisli_def, fastforce)
+
+lemma add_rem_commute2:
+fixes s
+assumes "i \<notin> is"  and "e1 \<noteq> e2"
+shows " (\<langle>Add i e1\<rangle> \<rhd> \<langle>Rem is e2\<rangle>) s = (\<langle>Rem is e2\<rangle> \<rhd> \<langle>Add i e1\<rangle>) s"
+	unfolding interpret_op_def op_elem_def kleisli_def using assms apply simp
+	by (smt bind_eq_Some_conv fst_conv fun_upd_other fun_upd_twist snd_conv)
+ 
+lemma add_rem_commute3:
+fixes s
+assumes "i \<notin> is" and "case snd s e of Some f \<Rightarrow> f \<subseteq> fst s e"
+shows " (\<langle>Add i e\<rangle> \<rhd> \<langle>Rem is e\<rangle>) s = (\<langle>Rem is e\<rangle> \<rhd> \<langle>Add i e\<rangle>) s"
+  unfolding interpret_op_def op_elem_def kleisli_def using assms apply simp apply (case_tac "snd s e = None") apply simp apply fastforce
+  	apply simp
+  by (smt Diff_eq_empty_iff bind_eq_Some_conv dual_order.trans fst_conv fun_upd_same fun_upd_upd insertI1 insert_Diff_if option.simps(4) option.simps(5) snd_conv subset_Compl_singleton)
+  	
+lemma (in orset) add_rem_commute:
+assumes "i \<notin> is" and "case snd s e2 of Some f \<Rightarrow> f \<subseteq> fst s e2"
+shows "(\<langle>Add i e1\<rangle> \<rhd> \<langle>Rem is e2\<rangle>) s = (\<langle>Rem is e2\<rangle> \<rhd> \<langle>Add i e1\<rangle>) s"
+	using assms add_rem_commute3[of "i" "is" "s" "e1"] add_rem_commute2 [of "i" "is" "e1" "e2" "s"]
+	by auto 
+
+  	
+lemma rem_rem_commute1:
+	assumes "e1 \<noteq> e2"
+	shows " (\<langle>Rem i1 e1\<rangle> \<rhd> \<langle>Rem i2 e2\<rangle>) s = (\<langle>Rem i2 e2\<rangle> \<rhd> \<langle>Rem i1 e1\<rangle>) s"
+	unfolding interpret_op_def kleisli_def op_elem_def apply (case_tac "snd s e1 = None", simp) 
+	 apply (smt assms bind_eq_Some_conv fst_conv fun_upd_other fun_upd_twist option.simps(4) snd_conv) apply simp
+proof clarify
+	fix y
+		have A1 :"((let before = fst s e1
+          in Some ((fst s)(e1 := before - i1), (snd s)
+                   (e1 := case snd s e1 of None \<Rightarrow> None | Some f \<Rightarrow> (case before - i1 = {} of True \<Rightarrow> None | False \<Rightarrow> Some (f - i1))))) \<bind>
+         (\<lambda>y. let before = fst y e2
+              in Some ((fst y)(e2 := before - i2), (snd y)
+                       (e2 := case snd y e2 of None \<Rightarrow> None | Some f \<Rightarrow> (case before - i2 = {} of True \<Rightarrow> None | False \<Rightarrow> Some (f - i2))))))
+ = Some ((fst s)(e1 := (fst s e1 - i1), e2 := (fst s e2 - i2)), 
+	(snd s)(
+		e1 := (case snd s e1 of None \<Rightarrow> None | Some f \<Rightarrow> (case fst s e1 - i1 = {} of True \<Rightarrow> None | False \<Rightarrow> Some (f - i1))), 
+		e2 := (case snd s e2 of None \<Rightarrow> None | Some f \<Rightarrow> (case fst s e2 - i2 = {} of True \<Rightarrow> None | False \<Rightarrow> Some (f - i2)))))"
+			by (smt assms bind_eq_Some_conv fst_conv fun_upd_other option.case_eq_if snd_conv)
+		have "(let before = fst s e2
+          in Some ((fst s)(e2 := before - i2), (snd s)
+                   (e2 := case snd s e2 of None \<Rightarrow> None | Some f \<Rightarrow> (case before - i2 = {} of True \<Rightarrow> None | False \<Rightarrow> Some (f - i2))))) \<bind>
+         (\<lambda>y. let before = fst y e1
+              in Some ((fst y)(e1 := before - i1), (snd y)
+                       (e1 := case snd y e1 of None \<Rightarrow> None | Some f \<Rightarrow> (case before - i1 = {} of True \<Rightarrow> None | False \<Rightarrow> Some (f - i1)))))
+	= Some ((fst s)(e1 := (fst s e1 - i1), e2 := (fst s e2 - i2)), 
+	(snd s)(
+		e1 := (case snd s e1 of None \<Rightarrow> None | Some f \<Rightarrow> (case fst s e1 - i1 = {} of True \<Rightarrow> None | False \<Rightarrow> Some (f - i1))), 
+		e2 := (case snd s e2 of None \<Rightarrow> None | Some f \<Rightarrow> (case fst s e2 - i2 = {} of True \<Rightarrow> None | False \<Rightarrow> Some (f - i2)))))"
+			by (smt assms bind.bind_lunit fst_conv fun_upd_other fun_upd_twist option.case_eq_if snd_conv)
+ 			
+		thus "(let before = fst s e1
+          in Some ((fst s)(e1 := before - i1), (snd s)
+                   (e1 := case snd s e1 of None \<Rightarrow> None | Some f \<Rightarrow> (case before - i1 = {} of True \<Rightarrow> None | False \<Rightarrow> Some (f - i1))))) \<bind>
+         (\<lambda>y. let before = fst y e2
+              in Some ((fst y)(e2 := before - i2), (snd y)
+                       (e2 := case snd y e2 of None \<Rightarrow> None | Some f \<Rightarrow> (case before - i2 = {} of True \<Rightarrow> None | False \<Rightarrow> Some (f - i2))))) =
+         (let before = fst s e2
+          in Some ((fst s)(e2 := before - i2), (snd s)
+                   (e2 := case snd s e2 of None \<Rightarrow> None | Some f \<Rightarrow> (case before - i2 = {} of True \<Rightarrow> None | False \<Rightarrow> Some (f - i2))))) \<bind>
+         (\<lambda>y. let before = fst y e1
+              in Some ((fst y)(e1 := before - i1), (snd y)
+                       (e1 := case snd y e1 of None \<Rightarrow> None | Some f \<Rightarrow> (case before - i1 = {} of True \<Rightarrow> None | False \<Rightarrow> Some (f - i1)))))"
+      using A1 by auto
+qed
+  	
+lemma rem_rem_commute2:
+assumes "(snd s) e1 = None"
+shows " (\<langle>Rem i1 e1\<rangle> \<rhd> \<langle>Rem i2 e1\<rangle>) s = (\<langle>Rem i2 e1\<rangle> \<rhd> \<langle>Rem i1 e1\<rangle>) s"
+unfolding interpret_op_def kleisli_def op_elem_def using assms apply simp by fastforce
+    	
+lemma rem_rem_commute3:
+assumes "(snd s) e1 \<noteq> None"
+shows " (\<langle>Rem i1 e1\<rangle> \<rhd> \<langle>Rem i2 e1\<rangle>) s = (\<langle>Rem i2 e1\<rangle> \<rhd> \<langle>Rem i1 e1\<rangle>) s"
+	unfolding interpret_op_def kleisli_def op_elem_def apply simp using assms 
+		apply (case_tac "(fst s e1) - i1 = {}", simp) 
+	 apply (smt Diff_eq_empty_iff Diff_subset bind.bind_lunit empty_subsetI fst_conv fun_upd_same fun_upd_upd option.simps(4) option.simps(5) snd_conv subset_trans)
+	  apply (case_tac "(fst s e1) - i2 = {}", simp)
+	 apply (smt Diff_disjoint Diff_eq Diff_eq_empty_iff Int_Diff bind.bind_lunit fst_conv fun_upd_same fun_upd_upd inf_commute option.simps(4) option.simps(5) snd_conv)
+	apply (case_tac "((fst s e1) - i1 - i2) = {}", simp add:  Diff_eq fun_upd_same Diff_subset) 
+	 apply (smt Diff_eq Int_assoc bind.bind_lunit fst_conv fun_upd_same fun_upd_upd inf_commute option.simps(5) snd_conv)
+	 proof clarify
+	fix y
+	assume A1: "fst s e1 - i1 \<noteq> {}"
+ "fst s e1 - i2 \<noteq> {}"
+ "fst s e1 - i1 - i2 \<noteq> {}"
+ "snd s e1 = Some y"
+	 
+have A2: "(let before = fst s e1
+          in Some ((fst s)(e1 := before - i1), (snd s)
+                   (e1 := case snd s e1 of None \<Rightarrow> None | Some f \<Rightarrow> (case before - i1 = {} of True \<Rightarrow> None | False \<Rightarrow> Some (f - i1))))) \<bind>
+         (\<lambda>y. let before = fst y e1
+              in Some ((fst y)(e1 := before - i2), (snd y)
+                       (e1 := case snd y e1 of None \<Rightarrow> None | Some f \<Rightarrow> (case before - i2 = {} of True \<Rightarrow> None | False \<Rightarrow> Some (f - i2)))))
+= Some (((fst s)(e1 := ((fst s e1) \<inter> - i1) \<inter> - i2)), (snd s) (e1 := Some(y - i1 - i2)) )" using A1 
+	by (simp add: diff_eq)
+		
+have "(let before = fst s e1
+          in Some ((fst s)(e1 := before - i2), (snd s)
+                   (e1 := case snd s e1 of None \<Rightarrow> None | Some f \<Rightarrow> (case before - i2 = {} of True \<Rightarrow> None | False \<Rightarrow> Some (f - i2))))) \<bind>
+         (\<lambda>y. let before = fst y e1
+              in Some ((fst y)(e1 := before - i1), (snd y)
+                       (e1 := case snd y e1 of None \<Rightarrow> None | Some f \<Rightarrow> (case before - i1 = {} of True \<Rightarrow> None | False \<Rightarrow> Some (f - i1)))))
+= Some (((fst s)(e1 := ((fst s e1) \<inter> - i1) \<inter> - i2)), (snd s) (e1 := Some(y - i1 - i2)) )" using A1 apply (simp add: diff_eq) 
+	by (smt Diff_Int2 Diff_Int_distrib2 diff_eq)
+ 
+ thus "(let before = fst s e1
+          in Some ((fst s)(e1 := before - i1), (snd s)
+                   (e1 := case snd s e1 of None \<Rightarrow> None | Some f \<Rightarrow> (case before - i1 = {} of True \<Rightarrow> None | False \<Rightarrow> Some (f - i1))))) \<bind>
+         (\<lambda>y. let before = fst y e1
+              in Some ((fst y)(e1 := before - i2), (snd y)
+                       (e1 := case snd y e1 of None \<Rightarrow> None | Some f \<Rightarrow> (case before - i2 = {} of True \<Rightarrow> None | False \<Rightarrow> Some (f - i2))))) =
+         (let before = fst s e1
+          in Some ((fst s)(e1 := before - i2), (snd s)
+                   (e1 := case snd s e1 of None \<Rightarrow> None | Some f \<Rightarrow> (case before - i2 = {} of True \<Rightarrow> None | False \<Rightarrow> Some (f - i2))))) \<bind>
+         (\<lambda>y. let before = fst y e1
+              in Some ((fst y)(e1 := before - i1), (snd y)
+                       (e1 := case snd y e1 of None \<Rightarrow> None | Some f \<Rightarrow> (case before - i1 = {} of True \<Rightarrow> None | False \<Rightarrow> Some (f - i1)))))"
+   using A1 A2 by auto
+qed
+	
+lemma rem_rem_commute:
+shows " \<langle>Rem i1 e1\<rangle> \<rhd> \<langle>Rem i2 e2\<rangle> = \<langle>Rem i2 e2\<rangle> \<rhd> \<langle>Rem i1 e1\<rangle>"
+proof
+	fix x
+	show "(\<langle>Rem i1 e1\<rangle> \<rhd> \<langle>Rem i2 e2\<rangle>) x = (\<langle>Rem i2 e2\<rangle> \<rhd> \<langle>Rem i1 e1\<rangle>) x"
+		using rem_rem_commute1[of e1 e2 i1 i2 x] 
+				  rem_rem_commute2[of x e1 i1 i2] 
+          rem_rem_commute3[of x e1 i1 i2]
+    by auto
+qed 
+
+lemma append_append_commute:
+shows " \<langle>Append e1 m1\<rangle> \<rhd> \<langle>Append e2 m2\<rangle> = \<langle>Append e2 m2\<rangle> \<rhd> \<langle>Append e1 m1\<rangle>"
+proof
+	fix x
+	show "(\<langle>Append e1 m1\<rangle> \<rhd> \<langle>Append e2 m2\<rangle>) x = (\<langle>Append e2 m2\<rangle> \<rhd> \<langle>Append e1 m1\<rangle>) x"
+		unfolding interpret_op_def kleisli_def op_elem_def apply simp
+		by (simp add: fun_upd_twist insert_commute option.case_eq_if)
+qed  
+
+lemma add_append_commute:
+	assumes "(snd x) e2 \<noteq> None"
+	shows " (\<langle>Add i e1\<rangle> \<rhd> \<langle>Append e2 m2\<rangle>) x = (\<langle>Append e2 m2\<rangle> \<rhd> \<langle>Add i e1\<rangle>) x"
+		unfolding interpret_op_def kleisli_def op_elem_def apply (case_tac "e1=e2") apply simp apply auto
+		apply (simp add: insert_commute) apply (simp add: option.case_eq_if) by (simp add: fun_upd_twist)
+			
+lemma rem_append_commute:
+	assumes  "m2 \<notin> is" and "case snd x e2 of Some f \<Rightarrow> f \<subseteq> fst x e2"
+	shows " (\<langle>Rem is e1\<rangle> \<rhd> \<langle>Append e2 m2\<rangle>) x = (\<langle>Append e2 m2\<rangle> \<rhd> \<langle>Rem is e1\<rangle>) x"
+		unfolding interpret_op_def kleisli_def op_elem_def apply (case_tac "e1 \<noteq> e2", simp) apply auto
+		 apply (smt bind_eq_Some_conv fst_conv fun_upd_other fun_upd_twist snd_conv) using assms 
+		apply (case_tac "(snd x e2) = None", simp) apply auto using assms apply simp 
+		apply (simp add: insert_Diff_if) using assms apply simp 
+		apply (simp add: Diff_eq option.case_eq_if)
+			by (smt Diff_eq Diff_eq_empty_iff bind.bind_lunit fst_conv fun_upd_apply fun_upd_upd option.discI option.sel snd_conv subset_trans)
+		  
+			
+lemma store_store_commute:
+	assumes "mn1 \<noteq> mo1" and "mn1 \<noteq> mo2" and "mn2 \<noteq> mo1" and "mn2 \<noteq> mo2"
+shows " (\<langle>Store e1 mo1 mn1\<rangle> \<rhd> \<langle>Store e2 mo2 mn2\<rangle>) x = (\<langle>Store e2 mo2 mn2\<rangle> \<rhd> \<langle>Store e1 mo1 mn1\<rangle>) x"
+	unfolding interpret_op_def kleisli_def op_elem_def apply (case_tac "e1\<noteq>e2") apply simp apply auto using assms
+		apply (simp add: fun_upd_twist) 
+	using assms(2) assms(3) apply fastforce by (smt Diff_disjoint Diff_insert Int_Diff assms(2) assms(3) insert_Diff_if insert_commute option.case_eq_if option.simps(5) singletonD)
+		
+lemma store_add_commute:
+assumes "i \<noteq> mo2"
+shows " (\<langle>Add i e1\<rangle> \<rhd> \<langle>Store e2 mo2 mn2\<rangle>) x = (\<langle>Store e2 mo2 mn2\<rangle> \<rhd> \<langle>Add i e1\<rangle>) x"
+	unfolding interpret_op_def kleisli_def op_elem_def apply (case_tac "e1=e2") apply simp apply auto 
+	apply (simp add: assms(1) insert_Diff_if insert_commute) 
+	apply (simp add: option.case_eq_if)
+	by (simp add: fun_upd_twist)
+
+lemma store_rem_commute:
+	assumes "mn2 \<notin> is" and "case snd x e1 of Some f \<Rightarrow> f \<subseteq> fst x e1"
+shows " (\<langle>Rem is e1\<rangle> \<rhd> \<langle>Store e2 mo2 mn2\<rangle>) x = (\<langle>Store e2 mo2 mn2\<rangle> \<rhd> \<langle>Rem is e1\<rangle>) x"
+	unfolding interpret_op_def kleisli_def op_elem_def apply (case_tac "e1\<noteq>e2") apply simp apply auto
+	using assms 
+	 apply (smt bind_eq_Some_conv fst_conv fun_upd_other fun_upd_twist snd_conv) using assms 
+	  	apply (case_tac "(snd x e2) = None", simp) apply auto using assms apply simp
+	 apply fastforce using assms apply simp 
+	  	apply (simp add: insert_Diff_if) using assms apply simp 
+	apply (simp add: Diff_eq option.case_eq_if) apply (case_tac "fst x e2 \<subseteq> is") apply simp 
+	apply (smt disjoint_eq_subset_Compl double_compl inf_le1 subset_trans) apply simp
+	by fastforce
+		
+lemma store_append_commute:
+	assumes "m \<noteq> mo2"
+shows " (\<langle>Append e1 m\<rangle> \<rhd> \<langle>Store e2 mo2 mn2\<rangle>) x = (\<langle>Store e2 mo2 mn2\<rangle> \<rhd> \<langle>Append e1 m\<rangle>) x"
+	unfolding interpret_op_def kleisli_def op_elem_def apply (case_tac "e1=e2") apply simp apply auto
+		apply (simp add: assms insert_Diff_if insert_commute) 
+	apply (simp add: assms insert_Diff_if insert_commute option.case_eq_if)
+	by (simp add: fun_upd_twist)
+
+
+		(*
+lemma expunge_expunge_commute:
+shows " (\<langle>Expunge e1 m1\<rangle> \<rhd> \<langle>Expunge e2 m2\<rangle>) x = (\<langle>Expunge e2 m2\<rangle> \<rhd> \<langle>Expunge e1 m1\<rangle>) x"
+	unfolding interpret_op_def kleisli_def op_elem_def apply (case_tac "e1=e2") apply simp apply auto
+	apply (case_tac "snd x e2 = None") by auto
+		
+lemma add_expunge_commute:
+shows " (\<langle>Add i e1\<rangle> \<rhd> \<langle>Expunge e2 m2\<rangle>) x = (\<langle>Expunge e2 m2\<rangle> \<rhd> \<langle>Add i e1\<rangle>) x"
+	unfolding interpret_op_def kleisli_def op_elem_def apply (case_tac "e1=e2") apply simp apply auto
+	apply (case_tac "snd x e2 = None") by auto
+		
+lemma rem_expunge_commute:
+	assumes "fst x e1 = {} \<Longrightarrow> snd x e1 = None"
+shows " (\<langle>Rem is e1 m\<rangle> \<rhd> \<langle>Expunge e2 m2\<rangle>) x = (\<langle>Expunge e2 m2\<rangle> \<rhd> \<langle>Rem is e1 m\<rangle>) x"
+	unfolding interpret_op_def kleisli_def op_elem_def apply (case_tac "e1=e2") apply simp apply auto
+	apply (case_tac "snd x e2 = None") apply simp apply simp nitpick
+		
+lemma append_expunge_commute:
+assumes "m1 \<noteq> m2"
+shows " (\<langle>Append e1 m1\<rangle> \<rhd> \<langle>Expunge e2 m2\<rangle>) x = (\<langle>Expunge e2 m2\<rangle> \<rhd> \<langle>Append e1 m1\<rangle>) x"
+	unfolding interpret_op_def kleisli_def op_elem_def apply (case_tac "e1=e2") apply simp apply auto
+	apply (case_tac "snd x e2 = None") apply auto by (simp add: assms insert_Diff_if)
+		
+lemma store_expunge_commute:
+assumes "m1n \<noteq> m2"
+shows " (\<langle>Store e1 m1o m1n\<rangle> \<rhd> \<langle>Expunge e2 m2\<rangle>) x = (\<langle>Expunge e2 m2\<rangle> \<rhd> \<langle>Store e1 m1o m1n\<rangle>) x"
+	unfolding interpret_op_def kleisli_def op_elem_def apply (case_tac "e1=e2") apply simp apply auto
+	apply (case_tac "snd x e2 = None") apply auto using assms by fastforce
+
+*)
+		
+lemma (in orset) apply_operations_never_fails:
+  assumes "xs prefix of i"
+  shows "apply_operations xs \<noteq> None"
+using assms proof(induction xs rule: rev_induct, clarsimp)
+  case (snoc x xs) thus ?case
+  proof (cases x)
+    case (Broadcast e) thus ?thesis
+      using snoc by force
+  next
+    case (Deliver e) thus ?thesis
+      using snoc by (simp, metis (no_types, lifting) bind.simps(2) interp_msg_def interpret_op_def prefix_of_appendD)
+  qed
+qed
+
+lemma (in orset) add_id_valid:
+  assumes "xs prefix of j"
+    and "Deliver (i1, Add i2 e) \<in> set xs"
+  shows "i1 = i2"
+proof -
+  have "\<exists>s. valid_behaviours s (i1, Add i2 e)"
+    using assms deliver_in_prefix_is_valid unfolding valid_behaviours_def by fastforce
+  thus ?thesis
+    by(simp add: valid_behaviours_def)
+qed
+	
+lemma (in orset) append_id_valid:
+  assumes "xs prefix of j"
+    and "Deliver (i1, Append e i2) \<in> set xs"
+  shows "i1 = i2"
+proof -
+  have "\<exists>s. valid_behaviours s (i1, Append e i2)"
+    using assms deliver_in_prefix_is_valid unfolding valid_behaviours_def by fastforce
+  thus ?thesis
+    by(simp add: valid_behaviours_def)
+qed
+	
+lemma (in orset) store_id_valid:
+  assumes "xs prefix of j"
+    and "Deliver (i1, Store e mo mn) \<in> set xs"
+  shows "i1 = mn"
+proof -
+  have "\<exists>s. valid_behaviours s (i1, Store e mo mn)"
+    using assms deliver_in_prefix_is_valid unfolding valid_behaviours_def by fastforce
+  thus ?thesis
+    by(simp add: valid_behaviours_def)
+qed
+
+definition (in orset) added_ids :: "('id \<times> ('id, 'b) operation) event list \<Rightarrow> 'b \<Rightarrow> 'id list" where
+  "added_ids es p \<equiv> List.map_filter (\<lambda>x. case x of 
+		Deliver (i, Add j e) \<Rightarrow> if e = p then Some j else None | 
+		Deliver (i, Append e j) \<Rightarrow> if e = p then Some j else None |
+		Deliver (i, Store e mo mn) \<Rightarrow> if e = p then Some mn else None |
+		_ \<Rightarrow> None) es"
+
+lemma (in orset) [simp]:
+  shows "added_ids [] e = []"
+  by (auto simp: added_ids_def map_filter_def)
+    
+lemma (in orset) [simp]:
+  shows "added_ids (xs @ ys) e = added_ids xs e @ added_ids ys e"
+    by (auto simp: added_ids_def map_filter_append)
+
+lemma (in orset) added_ids_Broadcast_collapse [simp]:
+  shows "added_ids ([Broadcast e]) e' = []"
+  by (auto simp: added_ids_def map_filter_append map_filter_def)
+    
+lemma (in orset) added_ids_Deliver_Rem_collapse [simp]:
+  shows "added_ids ([Deliver (i, Rem is e)]) e' = []"
+  by (auto simp: added_ids_def map_filter_append map_filter_def)
+    
+lemma (in orset) added_ids_Deliver_Add_diff_collapse [simp]:
+  shows "e \<noteq> e' \<Longrightarrow> added_ids ([Deliver (i, Add j e)]) e' = []"
+  by (auto simp: added_ids_def map_filter_append map_filter_def)
+  	
+lemma (in orset) added_ids_Deliver_Append_diff_collapse [simp]:
+  shows "e \<noteq> e' \<Longrightarrow> added_ids ([Deliver (i, Append e j)]) e' = []"
+  by (auto simp: added_ids_def map_filter_append map_filter_def)
+  	
+lemma (in orset) added_ids_Deliver_Store_diff_collapse [simp]:
+  shows "e \<noteq> e' \<Longrightarrow> added_ids ([Deliver (i, Store e mo j)]) e' = []"
+  by (auto simp: added_ids_def map_filter_append map_filter_def)
+    
+lemma (in orset) added_ids_Deliver_Add_same_collapse [simp]:
+  shows "added_ids ([Deliver (i, Add j e)]) e = [j]"
+  by (auto simp: added_ids_def map_filter_append map_filter_def)
+  	
+lemma (in orset) added_ids_Deliver_Append_same_collapse [simp]:
+  shows "added_ids ([Deliver (i, Append e j)]) e = [j]"
+  by (auto simp: added_ids_def map_filter_append map_filter_def)
+  	
+lemma (in orset) added_ids_Deliver_Store_same_collapse [simp]:
+  shows "added_ids ([Deliver (i, Store e mo j)]) e = [j]"
+  by (auto simp: added_ids_def map_filter_append map_filter_def)
+
+lemma (in orset) added_id_not_in_set:
+  assumes "i1 \<notin> set (added_ids [Deliver (i, Add i2 e)] e)"
+  shows "i1 \<noteq> i2"
+  using assms by simp
+  	
+lemma (in orset) added_id_not_in_set2:
+  assumes "i1 \<notin> set (added_ids [Deliver (i, Append e i2)] e)"
+  shows "i1 \<noteq> i2"
+  using assms by simp
+  	
+lemma (in orset) added_id_not_in_set3:
+  assumes "i1 \<notin> set (added_ids [Deliver (i, Store e mo i2)] e)"
+  shows "i1 \<noteq> i2"
+  using assms by simp
+ 
+  	
+declare [[ smt_timeout = 120 ]]
+	
+lemma (in orset) apply_operations_added_ids:
+  assumes "es prefix of j"
+    and "apply_operations es = Some f"
+  shows "(fst f) x \<subseteq> set (added_ids es x)"
+using assms proof (induct es arbitrary: f rule: rev_induct, force)
+  case (snoc x xs) thus ?case
+  proof (cases x)
+  	case (Broadcast x1)
+  	then show ?thesis apply simp using snoc apply simp by blast
+  next
+  	case (Deliver e)
+    moreover obtain a b where "e = (a, b)" by force
+    ultimately show ?thesis 
+      using snoc apply(case_tac b; clarsimp simp: interp_msg_def split: bind_splits)
+      apply (simp add: op_elem_def interpret_op_def)
+      	 apply (metis (no_types, lifting) added_id_not_in_set fst_conv fun_upd_other fun_upd_same insertE prefix_of_appendD subsetCE)
+      	apply (smt Diff_iff fst_conv fun_upd_other fun_upd_same interpret_op_def operation.case(2) option.sel prefix_of_appendD subset_iff)
+      unfolding interpret_op_def 
+      apply (smt Un_iff added_ids_Deliver_Append_same_collapse fst_conv fun_upd_other fun_upd_same list.simps(15) op_elem_def operation.simps(19) option.inject prefix_of_appendD set_empty subset_iff)
+      	
+      	apply (simp add: added_id_not_in_set3 op_elem_def prefix_of_appendD subsetCE)
+      	
+      by (smt Diff_subset added_id_not_in_set3 fst_conv fun_upd_other fun_upd_same insertE subsetCE)
+      	qed
+  qed
+    
+    
+lemma (in orset) Deliver_added_ids:
+  assumes "xs prefix of j"
+    and "i \<in> set (added_ids xs e)"
+  shows "Deliver (i, Add i e) \<in> set xs"
+using assms proof (induct xs rule: rev_induct, clarsimp)
+  case (snoc x xs) thus ?case
+  proof (cases x, force)
+    case (Deliver e')
+    moreover obtain a b where "e' = (a, b)" by force
+    ultimately show ?thesis
+      using snoc apply (case_tac b; clarsimp)
+       apply (metis added_ids_Deliver_Add_diff_collapse added_ids_Deliver_Add_same_collapse
+              empty_iff list.set(1) set_ConsD add_id_valid in_set_conv_decomp prefix_of_appendD)
+       apply force
+        sorry
+       (*done *) 
+  qed
+qed
+
+lemma (in orset) Broadcast_Deliver_prefix_closed:
+  assumes "xs @ [Broadcast (r, Rem ix e m)] prefix of j"
+    and "i \<in> ix"
+  shows "Deliver (i, Add i e) \<in> set xs"
+proof -  
+  obtain y where "apply_operations xs = Some y"
+    using assms broadcast_only_valid_msgs by blast
+  moreover hence "ix = fst y e"
+    by (metis (mono_tags, lifting) assms(1) broadcast_only_valid_msgs operation.case(2) option.simps(1)
+     valid_behaviours_def case_prodD)
+  ultimately show ?thesis
+    using assms Deliver_added_ids apply_operations_added_ids by blast
+qed
+
+lemma (in orset) Broadcast_Deliver_prefix_closed2:
+  assumes "xs prefix of j"
+    and "Broadcast (r, Rem ix e m) \<in> set xs"
+    and "i \<in> ix"
+  shows "Deliver (i, Add i e) \<in> set xs"
+using assms Broadcast_Deliver_prefix_closed by (induction xs rule: rev_induct; force)
+
+lemma (in orset) concurrent_add_remove_independent_technical:
+  assumes "i \<in> is"
+    and "xs prefix of j"
+    and "(i, Add i e) \<in> set (node_deliver_messages xs)" and "(ir, Rem is e m) \<in> set (node_deliver_messages xs)"
+  shows "hb (i, Add i e) (ir, Rem is e m)"
+proof -
+  obtain pre k where "pre@[Broadcast (ir, Rem is e m)] prefix of k"
+    using assms delivery_has_a_cause events_before_exist prefix_msg_in_history by blast
+  moreover hence "Deliver (i, Add i e) \<in> set pre"
+    using Broadcast_Deliver_prefix_closed assms(1) by auto
+  ultimately show ?thesis
+    using hb.intros(2) events_in_local_order by blast
+qed
+
+lemma (in orset) Deliver_Add_same_id_same_message:
+  assumes "Deliver (i, Add i e1) \<in> set (history j)" and "Deliver (i, Add i e2) \<in> set (history j)"
+  shows "e1 = e2"
+proof -
+  obtain pre1 pre2 k1 k2 where *: "pre1@[Broadcast (i, Add i e1)] prefix of k1" "pre2@[Broadcast (i, Add i e2)] prefix of k2"
+    using assms delivery_has_a_cause events_before_exist by meson
+  moreover hence "Broadcast (i, Add i e1) \<in> set (history k1)" "Broadcast (i, Add i e2) \<in> set (history k2)"
+    using node_histories.prefix_to_carriers node_histories_axioms by force+
+  ultimately show ?thesis
+    using msg_id_unique by fastforce
+qed
+
+lemma (in orset) ids_imply_messages_same:
+  assumes "i \<in> is"
+    and "xs prefix of j"
+    and "(i, Add i e1) \<in> set (node_deliver_messages xs)" and "(ir, Rem is e2 m) \<in> set (node_deliver_messages xs)"
+  shows "e1 = e2"
+proof -
+  obtain pre k where "pre@[Broadcast (ir, Rem is e2 m)] prefix of k"
+    using assms delivery_has_a_cause events_before_exist prefix_msg_in_history by blast
+  moreover hence "Deliver (i, Add i e2) \<in> set pre"
+    using Broadcast_Deliver_prefix_closed assms(1) by blast
+  moreover have "Deliver (i, Add i e1) \<in> set (history j)"
+    using assms(2) assms(3) prefix_msg_in_history by blast
+  ultimately show ?thesis
+    by (metis fst_conv msg_id_unique network.delivery_has_a_cause network_axioms operation.inject(1)
+        prefix_elem_to_carriers prefix_of_appendD prod.inject)
+qed
+
+corollary (in orset) concurrent_add_remove_independent:
+  assumes "\<not> hb (i, Add i e1) (ir, Rem is e2 m)" and "\<not> hb (ir, Rem is e2 m) (i, Add i e1)"
+    and "xs prefix of j"
+    and "(i, Add i e1) \<in> set (node_deliver_messages xs)" and "(ir, Rem is e2 m) \<in> set (node_deliver_messages xs)"
+  shows "i \<notin> is"
+  using assms ids_imply_messages_same concurrent_add_remove_independent_technical by fastforce  
+  	
+lemma (in orset) concurrent_operations_commute:
+  assumes "xs prefix of i"
+  shows "hb.concurrent_ops_commute (node_deliver_messages xs)"                     
+proof -
+  { fix a b x y
+    assume "(a, b) \<in> set (node_deliver_messages xs)"
+           "(x, y) \<in> set (node_deliver_messages xs)"
+           "hb.concurrent (a, b) (x, y)"
+    hence "interp_msg (a, b) \<rhd> interp_msg (x, y) = interp_msg (x, y) \<rhd> interp_msg (a, b)"
+      apply(unfold interp_msg_def, case_tac "b"; case_tac "y"; simp add: add_add_commute rem_rem_commute hb.concurrent_def)
+       apply (metis add_id_valid add_rem_commute assms concurrent_add_remove_independent prefix_contains_msg)+
+      done
+  } thus ?thesis
+    by(fastforce simp: hb.concurrent_ops_commute_def)
+qed
+  
+
+theorem (in orset) convergence:
+  assumes "set (node_deliver_messages xs) = set (node_deliver_messages ys)"
+      and "xs prefix of i" and "ys prefix of j"
+    shows "apply_operations xs = apply_operations ys"
+using assms by(auto simp add: apply_operations_def intro: hb.convergence_ext concurrent_operations_commute
+                node_deliver_messages_distinct hb_consistent_prefix)
+              
+context orset begin
+
+sublocale sec: strong_eventual_consistency weak_hb hb interp_msg
+  "\<lambda>ops.\<exists>xs i. xs prefix of i \<and> node_deliver_messages xs = ops" "(\<lambda>x.{}, \<lambda> x. None)"
+  apply(standard; clarsimp simp add: hb_consistent_prefix node_deliver_messages_distinct
+        concurrent_operations_commute)
+  unfolding hb.apply_operations_def node_deliver_messages_def interp_msg_def apply simp
+    apply (meson interpret_op_def)
+    by (metis drop_last_message trivial_network.node_deliver_messages_def)
+end
+end
+
+  
